@prefix dcat: <http://www.w3.org/ns/dcat#> .
@prefix dct: <http://purl.org/dc/terms/> .
@prefix dctype: <http://purl.org/dc/dcmitype/> .
@prefix foaf: <http://xmlns.com/foaf/0.1/> .
@prefix owl: <http://www.w3.org/2002/07/owl#> .
@prefix prov: <http://www.w3.org/ns/prov#> .
@prefix rdf: <http://www.w3.org/1999/02/22-rdf-syntax-ns#> .
@prefix rdfs: <http://www.w3.org/2000/01/rdf-schema#> .
@prefix sdo: <http://schema.org/> .
@prefix skos: <http://www.w3.org/2004/02/skos/core#> .
@prefix vcard: <http://www.w3.org/2006/vcard/ns#> .
@prefix xsd: <http://www.w3.org/2001/XMLSchema#> .

@prefix dcterms: <http://purl.org/dc/terms/> .
@prefix vann:    <http://purl.org/vocab/vann/> .
@prefix qb:      <http://purl.org/linked-data/cube#> .
@prefix daq:     <http://purl.org/eis/vocab/daq#> .
@prefix voaf:    <http://purl.org/vocommons/voaf#> .
@prefix oa:      <http://www.w3.org/ns/oa#> .
@prefix duv:     <http://www.w3.org/ns/duv#> .

@prefix dqv:     <http://www.w3.org/ns/dqv#> .

@prefix eodhqa: <https://eodatahub.org.uk/api/ontologies/qa/> .
@prefix eodhweblinks: <https://eodatahub.org.uk/api/ontologies/weblinks/> .


eodhqa:documentation
    a                   dqv:Category ;
    skos:prefLabel      "Documentation Review"@en ;
    skos:definition     "Quality information derived from the dataset's documentation"@en ;
    .

eodhqa:performance
    a                   dqv:Category ;
    skos:prefLabel      "Measured Performance"@en ;
    skos:definition     "Quality information derived from direct testing of product performance"@en
    .


# These dimensions correspond to the three columns of the 'Data Provider Documentation Review'
# matrix recommended by EDAP.
eodhqa:productInformation
    a                   dqv:Dimension;
    dqv:inCategory      eodhqa:documentation;
    skos:prefLabel      "Product Information"@en ;
    skos:definition     "Quality of basic descriptive information provided for the product"@en
    .

eodhqa:metrology
    a                   dqv:Dimension;
    dqv:inCategory      eodhqa:documentation;
    skos:prefLabel      "Metrology"@en ;
    skos:definition     "Metrics of the dataset's measurement quality"@en
    .

eodhqa:productGeneration
    a                   dqv:Dimension;
    dqv:inCategory      eodhqa:documentation;
    skos:prefLabel      "Product Generation"@en ;
    skos:definition     "Quality information about the processing steps used to produce the product"@en
    .

# These correspond to the Performance Specification section in the NPL mockup, or possibly also 
# the upper and lower halves of the EDAP Validation Summary.
eodhqa:radiometric
    a                   dqv:Dimension;
    dqv:inCategory      eodhqa:performance;
    skos:prefLabel      "Radiometric Uncertainty"@en ;
    skos:definition     "Measures of sensor measurement quality"@en
    .

eodhqa:geometric
    a                   dqv:Dimension;
    dqv:inCategory      eodhqa:performance;
    skos:prefLabel      "Geometric Uncertainty"@en ;
    skos:definition     "Measures of dataset positioning and coregistration accuracy"@en
    .



# These are the metrics in the Quality Information matrix / Documentation Review category.
eodhqa:productDetails
    a                       dqv:Metric;
    dqv:inDimension         eodhqa:productInformation;
    dqv:expectedDataType    xsd:string;
    skos:prefLabel          "Product Information"@en ;
    skos:definition         "Grading based on availability of basic descriptive information about the product"@en
    .

eodhqa:availabilityAndAccessibility
    a                       dqv:Metric;
    dqv:inDimension         eodhqa:productInformation;
    dqv:expectedDataType    xsd:string;
    skos:prefLabel          "Availability and Accessibility"@en ;
    skos:definition         "Grading based on whether FAIR principles are followed: Findability, Accessibility, Interoperability and Reusability"@en
    .

eodhqa:formatFlagsAndMetadata
    a                       dqv:Metric;
    dqv:inDimension         eodhqa:productInformation;
    dqv:expectedDataType    xsd:string;
    skos:prefLabel          "Product Format, Flags and Metadata"@en ;
    skos:definition         "Grading based on the product format, flags and metadata following documented or standardised formats"@en
    .

eodhqa:userDocumentation
    a                       dqv:Metric;
    dqv:inDimension         eodhqa:productInformation;
    dqv:expectedDataType    xsd:string;
    skos:prefLabel          "User Documentation"@en ;
    skos:definition         "Grading of product user guide and algorithm theoretical basis documentation"@en
    .




eodhqa:radiometricCalibration
    a                       dqv:Metric;
    dqv:inDimension         eodhqa:metrology;
    dqv:expectedDataType    xsd:string;
    skos:prefLabel          "Radiometric Calibration and Characterisation"@en;
    skos:definition         "Grading of the sensor's measurement calibration and characterisation process and documentation"@en
    .

eodhqa:geometricCalibration
    a                       dqv:Metric;
    dqv:inDimension         eodhqa:metrology;
    dqv:expectedDataType    xsd:string;
    skos:prefLabel          "Geometric Calibration and Characterisation"@en;
    skos:definition         "Grading of the sensor's geometric calibration and characterisation process and documentation"@en
    .

eodhqa:metrologicalTraceability
    a                       dqv:Metric;
    dqv:inDimension         eodhqa:metrology;
    dqv:expectedDataType    xsd:string;
    skos:prefLabel          "Metrological Traceability Documentation"@en;
    skos:definition         "Grading of the quality of the uncertainty tree diagram and traceability chain"@en
    .

eodhqa:uncertaintyCharacterisation
    a                       dqv:Metric;
    dqv:inDimension         eodhqa:metrology;
    dqv:expectedDataType    xsd:string;
    skos:prefLabel          "Uncertainty Characterisation"@en;
    skos:definition         "Grading of the availability and quality of estimates of measurement uncertainty"@en
    .

eodhqa:ancillaryData
    a                       dqv:Metric;
    dqv:inDimension         eodhqa:metrology;
    dqv:expectedDataType    xsd:string;
    skos:prefLabel          "Ancillary Data"@en;
    skos:definition         "Grading of the documentation, traceability and quality of ancillary data used for product generation"@en
    .


eodhqa:radiometricCalibrationAlgorithm
    a                       dqv:Metric;
    dqv:inDimension         eodhqa:productGeneration;
    dqv:expectedDataType    xsd:string;
    skos:prefLabel          "Radiometric Calibration Algorithm"@en;
    skos:definition         "Grading of the quality and documentation of the L1 calibration algorithm"@en
    .

eodhqa:geometricProcessing
    a                       dqv:Metric;
    dqv:inDimension         eodhqa:productGeneration;
    dqv:expectedDataType    xsd:string;
    skos:prefLabel          "Geometric Processing"@en;
    skos:definition         "Grading of the geometric processing methodology and documentation"@en
    .

eodhqa:retrievalAlgorithm
    a                       dqv:Metric;
    dqv:inDimension         eodhqa:productGeneration;
    dqv:expectedDataType    xsd:string;
    skos:prefLabel          "Retrieval Algorithm"@en;
    skos:definition         "Grading of the quality and documentation of the L2 retrieval algorithm"@en
    .

eodhqa:missionSpecificProcessing
    a                       dqv:Metric;
    dqv:inDimension         eodhqa:productGeneration;
    dqv:expectedDataType    xsd:string;
    skos:prefLabel          "Mission-specific Processing"@en;
    skos:definition         "Grading of the quality and documentation of any additional mission-specific processing steps"@en
    .


# These are the metrics in the Measured Performance category.
# This is probably not complete.
eodhqa:radiometricUncertainty
    a                       dqv:Metric;
    dqv:inDimension         eodhqa:radiometric;
    dqv:expectedDataType    xsd:double;
    skos:prefLabel          "Radiometric Uncertainty"@en;
    skos:definition         "?"@en
    .

eodhqa:snr
    a                       dqv:Metric ;
    dqv:inDimension         eodhqa:radiometric;
    dqv:expectedDataType    xsd:double;
    skos:prefLabel          "Signal-to-noise Ratio"@en;
    skos:altLabel           "SNR"@en;
    skos:definition         "Instrument signal-to-noise ratio"@en
    .

eodhqa:temporalStability
    a                       dqv:Metric ;
    dqv:inDimension         eodhqa:radiometric;
    dqv:expectedDataType    xsd:double;
    skos:prefLabel          "Temporal Stability"@en;
    skos:definition         "?"@en
    .

eodhqa:mtf
    a                       dqv:Metric ;
    dqv:inDimension         eodhqa:geometric;
    dqv:expectedDataType    xsd:double;
    skos:prefLabel          "MTF"@en;
    skos:definition         "?"@en
    .


###################################################################
# Grading scale used by EDAP
#
# First we have a generic grading scale then specific ones for each
# assessment. These are necessary because the definitions of what counts
# as 'good', etc., differ based on what is being assessed.
eodhqa:gradeNotAssessed
    a                       skos:Concept ;
    skos:prefLabel          "Not Assessed"@en;
    skos:definition         "Assessment was out-of-scope"@en
    .

eodhqa:gradeNotAssessable
    a                       skos:Concept ;
    skos:prefLabel          "Not Assessable"@en;
    skos:definition         "Assessed step not performed or information unavailable"@en
    .

eodhqa:gradeBasic
    a                       skos:Concept ;
    skos:prefLabel          "Basic"@en;
    skos:definition         "Alignment between validated and claimed performance, methods used and/or documentation provided fall short of being judged fit-for-purpose"@en
    .

eodhqa:gradeGood
    a                       skos:Concept ;
    skos:prefLabel          "Good"@en;
    skos:definition         "Alignment between validated and claimed performance, methods used and/or documentation provided are judged fit-for-purpose for most expected use cases"@en
    .

eodhqa:gradeExcellent
    a                       skos:Concept ;
    skos:prefLabel          "Excellent"@en;
    skos:definition         "Alignment between validated and claimed performance, methods used and/or documentation provided are judged fit-for-purpose for all expected use cases"@en
    .

eodhqa:gradeIdeal
    a                       skos:Concept ;
    skos:prefLabel          "Ideal"@en;
    skos:definition         "Alignment between validated and claimed performance, methods used and/or documentation provided are judged state-of-the art and easily fit-for-purpose in terms of stated performance"@en
    .

eodhqa:gradeScale
    a                       rdfs:Class ;
    a                       owl:Class ;
    a                       skos:OrderedCollection ;
    rdfs:label              "EDAP Generic Grading Scale"@en ;
    rdfs:comment            "The generic grading scale defined by EDAP. The specific meanings of each grade vary depending on the dimension being measured."@en;
    skos:memberList         (eodhqa:gradeNotAssessed eodhqa:gradeNotAssessable eodhqa:gradeBasic eodhqa:gradeGood eodhqa:gradeExcellent eodhqa:gradeIdeal)
    .



#########################
# Now we have a grading scale used for the compliance of measured performance
# with mission claims.
eodhqa:performanceGradeNotAssessable
    a                       skos:Concept ;
    skos:prefLabel          "Not Assessable"@en;
    skos:definition         "No validation activity performed."@en;
    skos:broader            eodhqa:gradeNotAssessable
    .

eodhqa:performanceGradeBasic
    a                       skos:Concept ;
    skos:prefLabel          "Basic"@en;
    skos:definition         "Claimed mission performance shows some agreement with validation results"@en;
    skos:broader            eodhqa:gradeBasic
    .

eodhqa:performanceGradeGood
    a                       skos:Concept ;
    skos:prefLabel          "Good"@en;
    skos:definition         "Claimed mission performance shows good agreement with validation results"@en;
    skos:broader            eodhqa:gradeGood
    .

eodhqa:performanceGradeExcellent
    a                       skos:Concept ;
    skos:prefLabel          "Excellent"@en;
    skos:definition         "Claimed mission performance shows excellent agreement with validation results. Analysis performed independently of the satellite mission owner"@en;
    skos:broader            eodhqa:gradeExcellent
    .

eodhqa:performanceGradeIdeal
    a                       skos:Concept ;
    skos:prefLabel          "Ideal"@en;
    skos:definition         "Claimed mission performance shows excellent agreement with validation results, measurement uncertainties also validated. Analysis performed independently of the satellite mission owner"@en;
    skos:broader            eodhqa:gradeIdeal
    .

eodhqa:performanceGradeScale
    a                       rdfs:Class ;
    a                       owl:Class ;
    a                       skos:OrderedCollection ;
    skos:broader            eodhqa:gradeScale;
    rdfs:label              "EDAP Grading Scale"@en ;
    rdfs:comment            "The generic grading scale defined by EDAP. The specific meanings of each grade vary depending on the dimension being measured."@en;
    skos:memberList         (eodhqa:gradeNotAssessed eodhqa:gradeNotAssessable eodhqa:gradeBasic eodhqa:gradeGood eodhqa:gradeExcellent eodhqa:gradeIdeal)
    .



#######################################
# For some results we get just pass/partial/fail
eodhqa:pass
    a                       skos:Concept ;
    skos:prefLabel          "Pass"@en;
    skos:definition         "Dataset passes check"@en
    .

eodhqa:partialPass
    a                       skos:Concept ;
    skos:prefLabel          "Partial Pass"@en;
    skos:definition         "Dataset partially passes check"@en
    .

eodhqa:fail
    a                       skos:Concept ;
    skos:prefLabel          "Fail"@en;
    skos:definition         "Dataset fails check"@en
    .

eodhqa:passPartialFailScale
    a                       rdfs:Class ;
    a                       owl:Class ;
    a                       skos:OrderedCollection ;
    rdfs:label              "Pass/partial pass/fail Grading Scale"@en ;
    rdfs:comment            "Simple pass, partial pass or fail scale."@en;
    skos:memberList         (eodhqa:fail eodhqa:partialPass eodhqa:pass)
    .



eodhqa:EODHQualityMeasurementDataset
    a                       owl:Class, rdfs:Class ;
    rdfs:label              "EODH Quality Measurement Dataset"@en ;
    rdfs:comment            "Represents a dataset of quality measurements following EODH conventions. A distinguishing feature is that these must be computed on exactly one dataset."@en ;
    rdfs:subClassOf         dqv:QualityMeasurementDataset
    .

eodhqa:datasetComputedOn
    a                       rdf:Property;
    rdfs:label              "computed on"@en ;
    rdfs:comment            "Refers to the resource (e.g., a dataset, a linkset, a graph, a set of triples) on which the quality measurement is performed."@en ;
    rdfs:domain             eodhqa:EODHQualityMeasurementDataset;
    rdfs:range              dcat:Dataset, dcat:Distribution;
    .

eodhqa:weblink
    a                       rdf:Property;
    rdfs:label              "link"@en ;
    rdfs:comment            "Link to more information about the quality measurement."@en ;
    rdfs:domain             eodhqa:EODHQualityMeasurementDataset, dqv:Metric;
    rdfs:range              eodhweblinks:Weblink;
    .

eodhqa:detailedResultsLink
    a                       eodhweblinks:RelationType;
    rdfs:label              "detailed results" ;
    rdfs:comment            "Links to a detailed report, in human readable form, which further describe a quality result."
    .

eodhqa:resultVisualisationLink
    a                       eodhweblinks:RelationType;
    rdfs:label              "visualisation" ;
    rdfs:comment            "Links to a visualisation of quality results."
    .

eodhqa:validityEnd
    a                       rdf:Property;
    rdfs:label              "validity end"@en ;
    rdfs:comment            "These quality results are considered valid until this date."@en ;
    rdfs:domain             eodhqa:EODHQualityMeasurementDataset;
    rdfs:range              xsd:dateTime;
    .
